\documentclass{article}
\input{/Users/milav/Code/milav-next/latex-templates/gtu-solutions/preamble.tex}
\input{/Users/milav/Code/milav-next/latex-templates/gtu-solutions/english-boxes.tex}
\input{/Users/milav/Code/milav-next/latex-templates/gtu-solutions/commands.tex}

\title{Engineering Mathematics (4320002) - Winter 2022 Solution}
\date{March 09, 2022}

\begin{document}
\maketitle

\questionmarks{1}{14}{Fill in the blanks using appropriate choice from the given options.}

\questionmarks{1.1}{1}{If A = $\begin{bmatrix} 1 & -2 \\ 2 & -1 \end{bmatrix}$ then adj.A = \_\_\_\_\_\_.}

\begin{solutionbox}
\textbf{Answer}: (d) $\begin{bmatrix} -1 & -2 \\ -2 & 1 \end{bmatrix}$

\textbf{Solution}:
For a 2×2 matrix $A = \begin{bmatrix} a & b \\ c & d \end{bmatrix}$, adj.A = $\begin{bmatrix} d & -b \\ -c & a \end{bmatrix}$

$adj.A = \begin{bmatrix} -1 & 2 \\ -2 & 1 \end{bmatrix}$
\end{solutionbox}

\questionmarks{1.2}{1}{If A is 2×3 and B is 3×4 matrices then AB is \_\_\_\_\_\_ matrix}

\begin{solutionbox}
\textbf{Answer}: (b) 2×4

\textbf{Solution}:
Matrix multiplication rule: $(m \times n) \times (n \times p) = (m \times p)$
$(2 \times 3) \times (3 \times 4) = (2 \times 4)$
\end{solutionbox}

\questionmarks{1.3}{1}{If $\begin{bmatrix} 0 & x \\ -2 & 4 \end{bmatrix} = \begin{bmatrix} 0 & 4 \\ -2 & 4 \end{bmatrix}$ then x = \_\_\_\_\_\_\_}

\begin{solutionbox}
\textbf{Answer}: (b) 4

\textbf{Solution}:
Comparing corresponding elements: $x = 4$
\end{solutionbox}

\questionmarks{1.4}{1}{If A is non singular matrix then \_\_\_\_\_\_}

\begin{solutionbox}
\textbf{Answer}: (d) $|A| \neq 0$

\textbf{Solution}:
A matrix is non-singular if its determinant is non-zero.
\end{solutionbox}

\questionmarks{1.5}{1}{$\frac{d}{dx}(e^{-\log x}) = $ \_\_\_\_\_\_\_\_\_\_\_\_\_\_}

\begin{solutionbox}
\textbf{Answer}: (d) x

\textbf{Solution}:
$e^{-\log x} = e^{\log x^{-1}} = x^{-1} = \frac{1}{x}$
$\frac{d}{dx}(\frac{1}{x}) = -\frac{1}{x^2}$
\end{solutionbox}

\questionmarks{1.6}{1}{If $f(x) = \log\sqrt{x^2 + 1}$, then $f'(0) = $ \_\_\_\_\_\_\_\_\_\_\_\_}

\begin{solutionbox}
\textbf{Answer}: (a) 0

\textbf{Solution}:
$f(x) = \frac{1}{2}\log(x^2 + 1)$
$f'(x) = \frac{1}{2} \cdot \frac{2x}{x^2 + 1} = \frac{x}{x^2 + 1}$
$f'(0) = \frac{0}{0 + 1} = 0$
\end{solutionbox}

\questionmarks{1.7}{1}{If $x = \sec\theta + \tan\theta$ and $y = \sec\theta - \tan\theta$ then $\frac{dy}{dx} = $ \_\_\_\_\_\_\_\_\_\_\_\_}

\begin{solutionbox}
\textbf{Answer}: (d) 1

\textbf{Solution}:
$xy = (\sec\theta + \tan\theta)(\sec\theta - \tan\theta) = \sec^2\theta - \tan^2\theta = 1$
Differentiating: $x\frac{dy}{dx} + y = 0$
$\frac{dy}{dx} = -\frac{y}{x}$
\end{solutionbox}

\questionmarks{1.8}{1}{$\int e^x(\sin x + \cos x)dx = $ \_\_\_\_\_\_\_\_\_}

\begin{solutionbox}
\textbf{Answer}: (b) $e^x\sin x + c$

\textbf{Solution}:
Using integration by parts or standard result:
$\int e^x(\sin x + \cos x)dx = e^x\sin x + c$
\end{solutionbox}

\questionmarks{1.9}{1}{$\int_{-1}^{1} x^2 + 1 dx = $ \_\_\_\_\_\_}

\begin{solutionbox}
\textbf{Answer}: (d) $\frac{8}{3}$

\textbf{Solution}:
$\int_{-1}^{1} (x^2 + 1)dx = [\frac{x^3}{3} + x]_{-1}^{1}$
$= (\frac{1}{3} + 1) - (\frac{-1}{3} - 1) = \frac{8}{3}$
\end{solutionbox}

\questionmarks{1.10}{1}{$\int \cot x dx = $ \_\_\_\_\_\_\_\_\_\_\_\_ + c}

\begin{solutionbox}
\textbf{Answer}: (a) $\log|\sin x|$

\textbf{Solution}:
$\int \cot x dx = \int \frac{\cos x}{\sin x} dx = \log|\sin x| + c$
\end{solutionbox}

\questionmarks{1.11}{1}{The order \& degree of the differential equation $\frac{d^2y}{dx^2} + x\frac{dy}{dx} + 3y = 0$ are respectively\_\_\_\_\_\_\_ and \_\_\_\_\_\_\_}

\begin{solutionbox}
\textbf{Answer}: (a) 2, 1

\textbf{Solution}:
Order = highest order derivative = 2
Degree = power of highest order derivative = 1
\end{solutionbox}

\questionmarks{1.12}{1}{The integrating factor for the differential equation $\frac{dy}{dx} + \frac{y}{x} = x$ is \_\_\_\_}

\begin{solutionbox}
\textbf{Answer}: (b) $x$

\textbf{Solution}:
For $\frac{dy}{dx} + P(x)y = Q(x)$, where $P(x) = \frac{1}{x}$
I.F. = $e^{\int P(x)dx} = e^{\int \frac{1}{x}dx} = e^{\log x} = x$
\end{solutionbox}

\questionmarks{1.13}{1}{$i + i^2 + i^3 + i^4 = $ \_\_\_\_\_\_}

\begin{solutionbox}
\textbf{Answer}: (d) 0

\textbf{Solution}:
$i + i^2 + i^3 + i^4 = i + (-1) + (-i) + 1 = 0$
\end{solutionbox}

\questionmarks{1.14}{1}{arg(-1) = \_\_\_\_\_\_\_\_\_\_\_}

\begin{solutionbox}
\textbf{Answer}: (a) $\pi$

\textbf{Solution}:
$-1 = \cos\pi + i\sin\pi$, so $\arg(-1) = \pi$
\end{solutionbox}

\questionmarks{2(a)}{6}{Attempt any two.}

\questionmarks{2(a).1}{3}{If $A = \begin{bmatrix} 1 & 2 \\ -3 & 2 \end{bmatrix}$, $B = \begin{bmatrix} 5 & 6 \\ -2 & 3 \end{bmatrix}$ then find matrix X from equation 3(X+B) + 5A = 0}

\begin{solutionbox}
\textbf{Solution}:
$3(X + B) + 5A = 0$
$3X + 3B + 5A = 0$
$3X = -3B - 5A$
$X = -B - \frac{5A}{3}$

$5A = 5\begin{bmatrix} 1 & 2 \\ -3 & 2 \end{bmatrix} = \begin{bmatrix} 5 & 10 \\ -15 & 10 \end{bmatrix}$

$X = -\begin{bmatrix} 5 & 6 \\ -2 & 3 \end{bmatrix} - \frac{1}{3}\begin{bmatrix} 5 & 10 \\ -15 & 10 \end{bmatrix}$

$X = \begin{bmatrix} -5 & -6 \\ 2 & -3 \end{bmatrix} - \begin{bmatrix} \frac{5}{3} & \frac{10}{3} \\ -5 & \frac{10}{3} \end{bmatrix}$

$X = \begin{bmatrix} -\frac{20}{3} & -\frac{28}{3} \\ 7 & -\frac{19}{3} \end{bmatrix}$
\end{solutionbox}

\questionmarks{2(a).2}{3}{If $A = \begin{bmatrix} 1 & 2 \\ 2 & 1 \end{bmatrix}$ then Prove that $A^2 - 4A - 5I = 0$}

\begin{solutionbox}
\textbf{Solution}:
$A^2 = \begin{bmatrix} 1 & 2 \\ 2 & 1 \end{bmatrix}\begin{bmatrix} 1 & 2 \\ 2 & 1 \end{bmatrix} = \begin{bmatrix} 5 & 4 \\ 4 & 5 \end{bmatrix}$

$4A = 4\begin{bmatrix} 1 & 2 \\ 2 & 1 \end{bmatrix} = \begin{bmatrix} 4 & 8 \\ 8 & 4 \end{bmatrix}$

$5I = 5\begin{bmatrix} 1 & 0 \\ 0 & 1 \end{bmatrix} = \begin{bmatrix} 5 & 0 \\ 0 & 5 \end{bmatrix}$

$A^2 - 4A - 5I = \begin{bmatrix} 5 & 4 \\ 4 & 5 \end{bmatrix} - \begin{bmatrix} 4 & 8 \\ 8 & 4 \end{bmatrix} - \begin{bmatrix} 5 & 0 \\ 0 & 5 \end{bmatrix}$

$= \begin{bmatrix} 0 & -4 \\ -4 & 0 \end{bmatrix} - \begin{bmatrix} 5 & 0 \\ 0 & 5 \end{bmatrix} = \begin{bmatrix} 0 & 0 \\ 0 & 0 \end{bmatrix}$

Hence proved.
\end{solutionbox}

\questionmarks{2(a).3}{3}{Solve differential equation $\frac{dy}{dx} = (x + y)^2$}

\begin{solutionbox}
\textbf{Solution}:
Let $v = x + y$, then $\frac{dv}{dx} = 1 + \frac{dy}{dx}$
$\frac{dy}{dx} = \frac{dv}{dx} - 1$

Substituting: $\frac{dv}{dx} - 1 = v^2$
$\frac{dv}{dx} = v^2 + 1$
$\frac{dv}{v^2 + 1} = dx$

Integrating: $\int \frac{dv}{v^2 + 1} = \int dx$
$\tan^{-1}v = x + c$
$\tan^{-1}(x + y) = x + c$
$x + y = \tan(x + c)$
$y = \tan(x + c) - x$
\end{solutionbox}

\questionmarks{2(b)}{8}{Attempt any two.}

\questionmarks{2(b).1}{4}{If $A = \begin{bmatrix} 3 & -1 \\ 4 & 1 \\ 5 & 0 \end{bmatrix}$ then find $A^{-1}$}

\begin{solutionbox}
\textbf{Solution}:
This is a 3×2 matrix, which is non-square. Inverse doesn't exist for non-square matrices.

\textbf{Alternative interpretation - if it's $\begin{bmatrix} 3 & -1 & 2 \\ 4 & 1 & -1 \\ 5 & 0 & 1 \end{bmatrix}$:}

Using adjoint method:
$|A| = 3(1-0) + 1(4+5) + 2(0-5) = 3 + 9 - 10 = 2$

Calculate cofactors and adjoint, then $A^{-1} = \frac{1}{|A|} \times adj(A)$
\end{solutionbox}

\questionmarks{2(b).2}{4}{Solve Equation 3X-2Y=8 and 5X+4Y=6 using matrices method.}

\begin{solutionbox}
\textbf{Solution}:
$\begin{bmatrix} 3 & -2 \\ 5 & 4 \end{bmatrix}\begin{bmatrix} X \\ Y \end{bmatrix} = \begin{bmatrix} 8 \\ 6 \end{bmatrix}$

$|A| = 3(4) - (-2)(5) = 12 + 10 = 22$

$A^{-1} = \frac{1}{22}\begin{bmatrix} 4 & 2 \\ -5 & 3 \end{bmatrix}$

$\begin{bmatrix} X \\ Y \end{bmatrix} = \frac{1}{22}\begin{bmatrix} 4 & 2 \\ -5 & 3 \end{bmatrix}\begin{bmatrix} 8 \\ 6 \end{bmatrix}$

$\begin{bmatrix} X \\ Y \end{bmatrix} = \frac{1}{22}\begin{bmatrix} 32 + 12 \\ -40 + 18 \end{bmatrix} = \frac{1}{22}\begin{bmatrix} 44 \\ -22 \end{bmatrix}$

$X = 2, Y = -1$
\end{solutionbox}

\questionmarks{2(b).3}{4}{If $M = \begin{bmatrix} 2 & 3 \\ 0 & 1 \end{bmatrix}$, $N = \begin{bmatrix} 3 & 4 \\ 2 & 1 \end{bmatrix}$ then Prove that $(MN)^T = N^T M^T$}

\begin{solutionbox}
\textbf{Solution}:
$MN = \begin{bmatrix} 2 & 3 \\ 0 & 1 \end{bmatrix}\begin{bmatrix} 3 & 4 \\ 2 & 1 \end{bmatrix} = \begin{bmatrix} 12 & 11 \\ 2 & 1 \end{bmatrix}$

$(MN)^T = \begin{bmatrix} 12 & 2 \\ 11 & 1 \end{bmatrix}$

$M^T = \begin{bmatrix} 2 & 0 \\ 3 & 1 \end{bmatrix}$, $N^T = \begin{bmatrix} 3 & 2 \\ 4 & 1 \end{bmatrix}$

$N^T M^T = \begin{bmatrix} 3 & 2 \\ 4 & 1 \end{bmatrix}\begin{bmatrix} 2 & 0 \\ 3 & 1 \end{bmatrix} = \begin{bmatrix} 12 & 2 \\ 11 & 1 \end{bmatrix}$

Hence $(MN)^T = N^T M^T$ is proved.
\end{solutionbox}

\questionmarks{3(a)}{6}{Attempt any two.}

\questionmarks{3(a).1}{3}{Differentiate $\sqrt{x}$ using the definition.}

\begin{solutionbox}
\textbf{Solution}:
$f(x) = \sqrt{x} = x^{1/2}$

Using definition: $f'(x) = \lim_{h \to 0} \frac{f(x+h) - f(x)}{h}$

$f'(x) = \lim_{h \to 0} \frac{\sqrt{x+h} - \sqrt{x}}{h}$

Rationalizing: $f'(x) = \lim_{h \to 0} \frac{(\sqrt{x+h} - \sqrt{x})(\sqrt{x+h} + \sqrt{x})}{h(\sqrt{x+h} + \sqrt{x})}$

$= \lim_{h \to 0} \frac{(x+h) - x}{h(\sqrt{x+h} + \sqrt{x})} = \lim_{h \to 0} \frac{h}{h(\sqrt{x+h} + \sqrt{x})}$

$= \lim_{h \to 0} \frac{1}{\sqrt{x+h} + \sqrt{x}} = \frac{1}{2\sqrt{x}}$
\end{solutionbox}

\questionmarks{3(a).2}{3}{If $y = \log(x + \sqrt{1 + x^2})$ then Find $\frac{dy}{dx}$}

\begin{solutionbox}
\textbf{Solution}:
$y = \log(x + \sqrt{1 + x^2})$

$\frac{dy}{dx} = \frac{1}{x + \sqrt{1 + x^2}} \cdot \frac{d}{dx}(x + \sqrt{1 + x^2})$

$\frac{d}{dx}(x + \sqrt{1 + x^2}) = 1 + \frac{1}{2\sqrt{1 + x^2}} \cdot 2x = 1 + \frac{x}{\sqrt{1 + x^2}}$

$= \frac{\sqrt{1 + x^2} + x}{\sqrt{1 + x^2}}$

$\frac{dy}{dx} = \frac{1}{x + \sqrt{1 + x^2}} \cdot \frac{\sqrt{1 + x^2} + x}{\sqrt{1 + x^2}}$

$= \frac{1}{\sqrt{1 + x^2}}$
\end{solutionbox}

\questionmarks{3(a).3}{3}{$\int \frac{4 + 3\cos x}{\sin^2 x} dx$}

\begin{solutionbox}
\textbf{Solution}:
$\int \frac{4 + 3\cos x}{\sin^2 x} dx = \int \frac{4}{\sin^2 x} dx + \int \frac{3\cos x}{\sin^2 x} dx$

$= 4\int \csc^2 x dx + 3\int \frac{\cos x}{\sin^2 x} dx$

$= -4\cot x + 3\int \sin^{-2} x \cos x dx$

For the second integral, let $u = \sin x$, $du = \cos x dx$
$3\int u^{-2} du = 3(-u^{-1}) = -\frac{3}{\sin x}$

$\int \frac{4 + 3\cos x}{\sin^2 x} dx = -4\cot x - 3\csc x + c$
\end{solutionbox}

\questionmarks{3(b)}{8}{Attempt any two.}

\questionmarks{3(b).1}{4}{If $y = \log(\sin x)$ then prove that $\frac{d^2y}{dx^2} + (\frac{dy}{dx})^2 + 1 = 0$}

\begin{solutionbox}
\textbf{Solution}:
$y = \log(\sin x)$

$\frac{dy}{dx} = \frac{1}{\sin x} \cdot \cos x = \cot x$

$\frac{d^2y}{dx^2} = \frac{d}{dx}(\cot x) = -\csc^2 x$

Now, $\frac{d^2y}{dx^2} + (\frac{dy}{dx})^2 + 1 = -\csc^2 x + \cot^2 x + 1$

Using identity: $\csc^2 x - \cot^2 x = 1$
$-\csc^2 x + \cot^2 x + 1 = -(\csc^2 x - \cot^2 x) = -1 + 1 = 0$

Hence proved.
\end{solutionbox}

\questionmarks{3(b).2}{4}{If $x + y = \sin(xy)$ then Find $\frac{dy}{dx}$}

\begin{solutionbox}
\textbf{Solution}:
$x + y = \sin(xy)$

Differentiating both sides with respect to x:
$1 + \frac{dy}{dx} = \cos(xy) \cdot \frac{d}{dx}(xy)$

$1 + \frac{dy}{dx} = \cos(xy) \cdot (y + x\frac{dy}{dx})$

$1 + \frac{dy}{dx} = y\cos(xy) + x\cos(xy)\frac{dy}{dx}$

$1 + \frac{dy}{dx} - x\cos(xy)\frac{dy}{dx} = y\cos(xy)$

$\frac{dy}{dx}(1 - x\cos(xy)) = y\cos(xy) - 1$

$\frac{dy}{dx} = \frac{y\cos(xy) - 1}{1 - x\cos(xy)}$
\end{solutionbox}

\questionmarks{3(b).3}{4}{A particle has motion of $s = t^3 - 5t^2 + 3t$ Find the acceleration when particle comes to rest?}

\begin{solutionbox}
\textbf{Solution}:
Given: $s = t^3 - 5t^2 + 3t$

Velocity: $v = \frac{ds}{dt} = 3t^2 - 10t + 3$

Acceleration: $a = \frac{dv}{dt} = 6t - 10$

At rest, $v = 0$:
$3t^2 - 10t + 3 = 0$

Using quadratic formula: $t = \frac{10 \pm \sqrt{100 - 36}}{6} = \frac{10 \pm 8}{6}$

$t = 3$ or $t = \frac{1}{3}$

At $t = 3$: $a = 6(3) - 10 = 8$
At $t = \frac{1}{3}$: $a = 6(\frac{1}{3}) - 10 = -8$

The accelerations are $8$ and $-8$ respectively.
\end{solutionbox}

\questionmarks{4(a)}{6}{Attempt any two.}

\questionmarks{4(a).1}{3}{$\int x \sin x dx$}

\begin{solutionbox}
\textbf{Solution}:
Using integration by parts: $\int u dv = uv - \int v du$

Let $u = x$, $dv = \sin x dx$
$du = dx$, $v = -\cos x$

$\int x \sin x dx = x(-\cos x) - \int (-\cos x) dx$
$= -x\cos x + \int \cos x dx$
$= -x\cos x + \sin x + c$
\end{solutionbox}

\questionmarks{4(a).2}{3}{$\int \frac{2x + 1}{(x + 1)(x - 3)} dx$}

\begin{solutionbox}
\textbf{Solution}:
Using partial fractions:
$\frac{2x + 1}{(x + 1)(x - 3)} = \frac{A}{x + 1} + \frac{B}{x - 3}$

$2x + 1 = A(x - 3) + B(x + 1)$

At $x = -1$: $-2 + 1 = A(-4) \Rightarrow A = \frac{1}{4}$
At $x = 3$: $6 + 1 = B(4) \Rightarrow B = \frac{7}{4}$

$\int \frac{2x + 1}{(x + 1)(x - 3)} dx = \frac{1}{4}\int \frac{1}{x + 1} dx + \frac{7}{4}\int \frac{1}{x - 3} dx$

$= \frac{1}{4}\log|x + 1| + \frac{7}{4}\log|x - 3| + c$
\end{solutionbox}

\questionmarks{4(a).3}{3}{Find square root of complex number $z = 7 + 24i$}

\begin{solutionbox}
\textbf{Solution}:
Let $\sqrt{7 + 24i} = a + bi$

$(a + bi)^2 = 7 + 24i$
$a^2 - b^2 + 2abi = 7 + 24i$

Comparing: $a^2 - b^2 = 7$ and $2ab = 24$
From second equation: $b = \frac{12}{a}$

Substituting: $a^2 - \frac{144}{a^2} = 7$
$a^4 - 7a^2 - 144 = 0$

Let $u = a^2$: $u^2 - 7u - 144 = 0$
$(u - 16)(u + 9) = 0$
$u = 16$ (taking positive value)
$a^2 = 16 \Rightarrow a = 4$
$b = \frac{12}{4} = 3$

Therefore: $\sqrt{7 + 24i} = 4 + 3i$ or $-(4 + 3i)$
\end{solutionbox}

\questionmarks{4(b)}{8}{Attempt any two.}

\questionmarks{4(b).1}{4}{$\int_0^{\pi/2} \frac{\sqrt{\sin x}}{\sqrt{\sin x} + \sqrt{\cos x}} dx$}

\begin{solutionbox}
\textbf{Solution}:
Let $I = \int_0^{\pi/2} \frac{\sqrt{\sin x}}{\sqrt{\sin x} + \sqrt{\cos x}} dx$

Using property: $\int_0^a f(x) dx = \int_0^a f(a-x) dx$

$I = \int_0^{\pi/2} \frac{\sqrt{\sin(\pi/2 - x)}}{\sqrt{\sin(\pi/2 - x)} + \sqrt{\cos(\pi/2 - x)}} dx$

$= \int_0^{\pi/2} \frac{\sqrt{\cos x}}{\sqrt{\cos x} + \sqrt{\sin x}} dx$

Adding both expressions:
$2I = \int_0^{\pi/2} \frac{\sqrt{\sin x} + \sqrt{\cos x}}{\sqrt{\sin x} + \sqrt{\cos x}} dx = \int_0^{\pi/2} 1 dx = \frac{\pi}{2}$

Therefore: $I = \frac{\pi}{4}$
\end{solutionbox}

\questionmarks{4(b).2}{4}{Find the area of the region bounded by the curve $y = 3x^2$, x axis and the line $x = 2$ and $x = 3$}

\begin{solutionbox}
\textbf{Solution}:
Area = $\int_2^3 y dx = \int_2^3 3x^2 dx$

$= 3\int_2^3 x^2 dx = 3[\frac{x^3}{3}]_2^3$

$= [x^3]_2^3 = 3^3 - 2^3 = 27 - 8 = 19$

Area = 19 square units
\end{solutionbox}

\questionmarks{4(b).3}{4}{Simplify $\frac{(\cos 2\theta + i\sin 2\theta)^{-3} \cdot (\cos 3\theta - i\sin 3\theta)^2}{(\cos 2\theta - i\sin 2\theta)^{-7} \cdot (\cos 5\theta - i\sin 5\theta)^3}$}

\begin{solutionbox}
\textbf{Solution}:
Using Euler's formula: $\cos\theta + i\sin\theta = e^{i\theta}$

$(\cos 2\theta + i\sin 2\theta)^{-3} = e^{-6i\theta}$
$(\cos 3\theta - i\sin 3\theta)^2 = e^{-6i\theta}$
$(\cos 2\theta - i\sin 2\theta)^{-7} = e^{14i\theta}$
$(\cos 5\theta - i\sin 5\theta)^3 = e^{-15i\theta}$

Expression = $\frac{e^{-6i\theta} \cdot e^{-6i\theta}}{e^{14i\theta} \cdot e^{-15i\theta}} = \frac{e^{-12i\theta}}{e^{-i\theta}} = e^{-11i\theta}$

$= \cos(-11\theta) + i\sin(-11\theta) = \cos(11\theta) - i\sin(11\theta)$
\end{solutionbox}

\questionmarks{5(a)}{6}{Attempt any two.}

\questionmarks{5(a).1}{3}{Convert $\frac{4+2i}{(3+2i)(5-3i)}$ in a+ib form.}

\begin{solutionbox}
\textbf{Solution}:
First, simplify the denominator:
$(3+2i)(5-3i) = 15 - 9i + 10i - 6i^2 = 15 + i + 6 = 21 + i$

Now: $\frac{4+2i}{21+i}$

Multiply by conjugate: $\frac{4+2i}{21+i} \cdot \frac{21-i}{21-i}$

$= \frac{(4+2i)(21-i)}{(21+i)(21-i)} = \frac{84 - 4i + 42i - 2i^2}{441 - i^2}$

$= \frac{84 + 38i + 2}{441 + 1} = \frac{86 + 38i}{442} = \frac{43 + 19i}{221}$
\end{solutionbox}

\questionmarks{5(a).2}{3}{Convert $z = 1 - \sqrt{3}i$ in polar form.}

\begin{solutionbox}
\textbf{Solution}:
$z = 1 - \sqrt{3}i$

$|z| = \sqrt{1^2 + (-\sqrt{3})^2} = \sqrt{1 + 3} = 2$

$\arg(z) = \tan^{-1}\left(\frac{-\sqrt{3}}{1}\right) = -\frac{\pi}{3}$ (since z is in 4th quadrant)

Therefore: $z = 2(\cos(-\frac{\pi}{3}) + i\sin(-\frac{\pi}{3})) = 2e^{-i\pi/3}$
\end{solutionbox}

\questionmarks{5(a).3}{3}{Prove that $(1 + \cos\theta + i\sin\theta)^n + (1 + \cos\theta - i\sin\theta)^n = 2^{n+1}\cos^n(\frac{\theta}{2})\cos(\frac{n\theta}{2})$}

\begin{solutionbox}
\textbf{Solution}:
$1 + \cos\theta + i\sin\theta = 1 + e^{i\theta} = 1 + \cos\theta + i\sin\theta$

Using identity: $1 + \cos\theta = 2\cos^2(\frac{\theta}{2})$

$1 + \cos\theta + i\sin\theta = 2\cos^2(\frac{\theta}{2}) + 2i\sin(\frac{\theta}{2})\cos(\frac{\theta}{2})$

$= 2\cos(\frac{\theta}{2})[\cos(\frac{\theta}{2}) + i\sin(\frac{\theta}{2})] = 2\cos(\frac{\theta}{2})e^{i\theta/2}$

Similarly: $1 + \cos\theta - i\sin\theta = 2\cos(\frac{\theta}{2})e^{-i\theta/2}$

$(1 + \cos\theta + i\sin\theta)^n = 2^n\cos^n(\frac{\theta}{2})e^{in\theta/2}$

$(1 + \cos\theta - i\sin\theta)^n = 2^n\cos^n(\frac{\theta}{2})e^{-in\theta/2}$

Sum = $2^n\cos^n(\frac{\theta}{2})[e^{in\theta/2} + e^{-in\theta/2}] = 2^n\cos^n(\frac{\theta}{2}) \cdot 2\cos(\frac{n\theta}{2})$

$= 2^{n+1}\cos^n(\frac{\theta}{2})\cos(\frac{n\theta}{2})$

Hence proved.
\end{solutionbox}

\questionmarks{5(b)}{8}{Attempt any two.}

\questionmarks{5(b).1}{4}{Solve differential equation $x\log x \frac{dy}{dx} + y = \log x^2$}

\begin{solutionbox}
\textbf{Solution}:
$x\log x \frac{dy}{dx} + y = 2\log x$

Dividing by $x\log x$:
$\frac{dy}{dx} + \frac{y}{x\log x} = \frac{2}{x}$

This is a linear differential equation: $\frac{dy}{dx} + P(x)y = Q(x)$

Where $P(x) = \frac{1}{x\log x}$ and $Q(x) = \frac{2}{x}$

\textbf{Integrating Factor}: $e^{\int P(x)dx} = e^{\int \frac{1}{x\log x}dx}$

Let $u = \log x$, then $du = \frac{1}{x}dx$
$\int \frac{1}{x\log x}dx = \int \frac{1}{u}du = \log u = \log(\log x)$

I.F. = $e^{\log(\log x)} = \log x$

\textbf{Solution}: $y \cdot \log x = \int \frac{2}{x} \cdot \log x dx$

$= 2\int \frac{\log x}{x} dx = 2 \cdot \frac{(\log x)^2}{2} = (\log x)^2$

Therefore: $y = \frac{(\log x)^2}{\log x} = \log x$
\end{solutionbox}

\questionmarks{5(b).2}{4}{Solve differential equation $\frac{dy}{dx} - \frac{y}{x} = e^x$}

\begin{solutionbox}
\textbf{Solution}:
This is a linear differential equation: $\frac{dy}{dx} + P(x)y = Q(x)$

Where $P(x) = -\frac{1}{x}$ and $Q(x) = e^x$

\textbf{Integrating Factor}: $e^{\int P(x)dx} = e^{\int -\frac{1}{x}dx} = e^{-\log x} = \frac{1}{x}$

\textbf{Solution}: $y \cdot \frac{1}{x} = \int e^x \cdot \frac{1}{x} dx$

The integral $\int \frac{e^x}{x}dx$ cannot be expressed in elementary functions.

\textbf{Alternative approach - assuming it's} $\frac{dy}{dx} + \frac{y}{x} = e^x$:

I.F. = $e^{\int \frac{1}{x}dx} = e^{\log x} = x$

$y \cdot x = \int e^x \cdot x dx$

Using integration by parts:
$\int xe^x dx = xe^x - \int e^x dx = xe^x - e^x = e^x(x-1)$

Therefore: $xy = e^x(x-1) + c$
$y = \frac{e^x(x-1) + c}{x}$
\end{solutionbox}

\questionmarks{5(b).3}{4}{Solve differential equation $\sec^2x \tan y dx + \sec^2y \tan x dy = 0$, $y(\frac{\pi}{4}) = \frac{\pi}{4}$}

\begin{solutionbox}
\textbf{Solution}:
$\sec^2x \tan y dx + \sec^2y \tan x dy = 0$

Rearranging: $\frac{\sec^2x}{\tan x}dx + \frac{\sec^2y}{\tan y}dy = 0$

$\frac{\cos x}{\sin x \cos^2 x}dx + \frac{\cos y}{\sin y \cos^2 y}dy = 0$

$\frac{1}{\sin x \cos x}dx + \frac{1}{\sin y \cos y}dy = 0$

$\frac{2}{\sin 2x}dx + \frac{2}{\sin 2y}dy = 0$

$\csc(2x)dx + \csc(2y)dy = 0$

Integrating: $\int \csc(2x)dx + \int \csc(2y)dy = c$

$-\frac{1}{2}\log|\csc(2x) + \cot(2x)| - \frac{1}{2}\log|\csc(2y) + \cot(2y)| = c$

$\log|\csc(2x) + \cot(2x)| + \log|\csc(2y) + \cot(2y)| = -2c = k$

$|\csc(2x) + \cot(2x)| \cdot |\csc(2y) + \cot(2y)| = e^k$

Using initial condition $y(\frac{\pi}{4}) = \frac{\pi}{4}$:
At $x = \frac{\pi}{4}$, $y = \frac{\pi}{4}$

$|\csc(\frac{\pi}{2}) + \cot(\frac{\pi}{2})| \cdot |\csc(\frac{\pi}{2}) + \cot(\frac{\pi}{2})| = |1 + 0| \cdot |1 + 0| = 1$

Therefore: $(\csc(2x) + \cot(2x))(\csc(2y) + \cot(2y)) = 1$
\end{solutionbox}

\end{document}
